src/proof/kubernetes_model/update.v
@@ -1,0 +1,42 @@
+From New.proof Require Import prelude empty_ffi.
+From New.proof.kubernetes_model Require Export inv common.
+
+Section proof.
+Context `{hG: !heapGS Σ} {go_ctx: GoContext}.
+Context `{!kubernetesModelG Σ}.
+
+Lemma wp_State__update_au γ l kind namespace i kobj :
+  ∀ Φ,
+    is_pkg_init apimodel ∗
+    is_kubernetes γ l ∗
+    "%Hvalid" ∷ ⌜ KObjectV.valid kobj ⌝ ∗
+    "%Hkind_matches" ∷ ⌜ kind = KObjectV.kind kobj ⌝ ∗
+    "%Hns_matches" ∷ ⌜ namespace = (KObjectV.objectmeta kobj).(ObjectMetaV.Namespace') ⌝ ∗
+    "Hdeepown_i" ∷ KObjectV.deepown_i i kobj 1 ∗
+    ( |={⊤,∅}=> ∃ key uid kmeta kspec,
+      "Hown_meta_frag" ∷ own_meta_frag γ key uid 1 kmeta ∗
+      "Hown_spec_frag" ∷ own_spec_frag γ key uid 1 kspec ∗
+      "%Hkey_eq" ∷ ⌜ key = KObjectV.key kobj ⌝ ∗
+      "%Huid_eq" ∷ ⌜ uid = (KObjectV.objectmeta kobj).(ObjectMetaV.UID') ⌝ ∗
+      "%Hvalid_meta_update" ∷ ⌜ ObjectMetaV.valid_simple_update kmeta (KObjectV.objectmeta kobj) ⌝ ∗
+      "%Hvalid_spec_update" ∷ ⌜ ObjectSpecV.valid_update kspec (KObjectV.spec kobj) ⌝ ∗
+      (* Hno_deletion_timestamp ensures that the update doesn't delete the object *)
+      "%Hno_deletion_timestamp" ∷ ⌜ kmeta.(ObjectMetaV.DeletionTimestamp') = None ⌝ ∗
+      "Hclose" ∷ (
+          ∀ i' err kobj',
+            ( (⌜ err = interface.nil ⌝ ∗
+                ⌜ ObjectMetaV.updated (KObjectV.objectmeta kobj) (KObjectV.objectmeta kobj') ⌝ ∗
+                ⌜ ObjectSpecV.updated (KObjectV.spec kobj) (KObjectV.spec kobj') ⌝ ∗
+                KObjectV.deepown_i i' kobj' 1 ∗
+                own_meta_frag γ key uid 1 (KObjectV.objectmeta kobj') ∗
+                own_spec_frag γ key uid 1 (KObjectV.spec kobj')) ∨
+              (⌜ err ≠ interface.nil ⌝ ∗
+                own_meta_frag γ key uid 1 kmeta ∗
+                own_spec_frag γ key uid 1 kspec)
+            )
+              ={∅,⊤}=∗ ▷ Φ (#i', #err)%V
+      )%I
+    ) -∗ WP l @ (ptrT.id apimodel.State.id) @ "update" #kind #namespace #i {{ Φ }}.
+Proof. Admitted.
+
+End proof.
